Cslib/Computability/Machines/MultiTapeTuring/TapeView.lean
@@ -124,11 +124,18 @@ public def appendPath (tv : TapeView) (idx : ℕ)
     (h : (tv.current.atPath [idx]).isSome) : TapeView :=
   ⟨tv.data, tv.path ++ [idx], tv.headPos, by simpa using h⟩
 
+-- TODO rename `appendToPath`
+
 /-- Like `appendPath` but always sets `headPos` to `.leftEnd`. -/
 @[expose, simp]
 public def appendPath' (tv : TapeView) (idx : ℕ)
     (h : (tv.current.atPath [idx]).isSome) : TapeView :=
   ⟨tv.data, tv.path ++ [idx], .leftEnd, by simpa using h⟩
+
+@[expose, simp]
+public def appendPath'' (tv : TapeView) (path : List ℕ)
+    (h : (tv.current.atPath path).isSome) : TapeView :=
+  ⟨tv.data, tv.path ++ path, .leftEnd, by simpa using h⟩
 
 /-- Copy the `headPos` from `tv'` into `tv`, keeping all other fields. -/
 @[expose]
